Start on command calculus soundness

theories/Sat.v
@@ -2,16 +2,130 @@ Require Import Blech.Spec.
 Require Blech.Map.
 Require Import Blech.SpecNotations.
 
-Require Import Coq.Classes.SetoidClass.
+Require Blech.Context.
+Require Blech.Term.
+
+Require Import FunInd.
 
 Import IfNotations.
 
-Theorem id_fanout:
-  forall v t,
-  ⊢ v in t ->
-  let x := 0 in
-  Map.empty ⊢ (E_all x t (E_var x)) [ v_fanout v v ].
-Proof using.
-  repeat econstructor.
-  auto.
-Qed.
+Definition eq_type (x y: type): {x = y} + {x <> y}.
+Proof.
+  decide equality.
+Defined.
+
+Definition eq_term (x y: term): {x = y} + {x <> y}.
+Proof.
+  decide equality.
+Defined.
+
+Function typecheck (Γ: environment) (Δ: seq) (c: command): option (environment * context * term) :=
+  match c with
+  | c_var y =>
+      if Map.Env.find y Δ is Some (E, v)
+      then
+        Some (Γ, E, v)
+      else
+        None
+  | c_abs x t y v c =>
+      if typecheck (Map.add x t Γ) (Map.add y (E_var x, v) Δ) c is Some (Γ', E', v')
+      then
+        if Term.typecheck v is Some t'
+        then
+          if eq_type t t'
+          then
+            if Term.typecheck v' is Some t1
+            then
+              if Context.typecheck (Map.add x t Γ) E' is Some (Γ'', t1')
+              then
+                if eq_type t1 t1'
+                then
+                  Some (Map.minus x Γ', E_all x t E', v_fanout v v')
+                else
+                  None
+              else
+                None
+            else
+              None
+          else
+            None
+        else
+          None
+      else
+        None
+  | c_app c0 c1 =>
+      (* FIXME normalize ? *)
+      if typecheck Γ Δ c0 is Some (Γ', E0, v_fanout v0 v1)
+      then
+        if typecheck Γ Δ c1 is Some (Γ'', E1, v0')
+        then
+          if eq_term v0 v0'
+          then
+            Some (Map.merge Γ' Γ'', E_app E0 E1, v1)
+          else
+            None
+        else
+          None
+      else
+        None
+  end.
+
+Theorem typecheck_sound:
+  forall Γ Δ c Γ' E v,
+    typecheck Γ Δ c = Some (Γ', E, v) -> Jsat Γ Δ c E v.
+Proof.
+  intros Γ Δ c.
+  generalize dependent Δ.
+  generalize dependent Γ.
+  induction c.
+  all: cbn.
+  all: intros ? ? ? ? ? p.
+  - destruct (Map.Env.find y Δ).
+    2: discriminate.
+    destruct p0.
+    inversion p.
+    subst.
+    admit.
+  - destruct (typecheck (Map.add x t Γ) (Map.add y (E_var x, v0) Δ) c) eqn:q0.
+    2: discriminate.
+    destruct p0.
+    destruct p0.
+    destruct (Term.typecheck v0) eqn:q1.
+    2: discriminate.
+    destruct (eq_type t t1).
+    2: discriminate.
+    subst.
+    destruct (Term.typecheck t0) eqn:q2.
+    2: discriminate.
+    destruct (Context.typecheck (Map.add x t1 Γ) c0) eqn:q3.
+    2: discriminate.
+    destruct p0.
+    destruct (eq_type t t2).
+    2: discriminate.
+    subst.
+    inversion p.
+    subst.
+    econstructor.
+    all: eauto.
+    all: try apply Term.typecheck_sound.
+    all: eauto.
+    apply (Context.typecheck_sound (Map.add x t1 Γ)).
+    rewrite q3.
+    admit.
+  - destruct (typecheck Γ Δ c1) eqn:q1.
+    2: discriminate.
+    destruct p0.
+    destruct p0.
+    destruct t.
+    all: try discriminate.
+    destruct (typecheck Γ Δ c2) eqn:q2.
+    2: discriminate.
+    destruct p0.
+    destruct p0.
+    destruct (eq_term t1 t).
+    2: discriminate.
+    subst.
+    inversion p.
+    subst.
+    admit.
+Admitted.
