theories/SpecNotations.v
@@ -8,4 +8,4 @@ Notation "⊢ v 'in' t" := (Jv v t) (at level 90).
 Notation "v0 ~> v1" := (step_v v0 v1) (at level 90).
 Notation "v0 *~> v1" := (multi_v v0 v1) (at level 90).
 
-Notation "Δ ⊢ E [ v ]" := (Jsat Δ E v) (at level 90).
+Notation "Γ ; Δ ⊢ c 'in' E [ v ]" := (Jsat Γ Δ c E v) (at level 90).
